Implement stateful serializers for integers: aux

src/lowparse/LowParse.Low.Int.Aux.fst
@@ -36,3 +36,42 @@ let parse32_u8 : parser32 parse_u8 =
     decode_u8
     ()
     (fun b -> B.index b 0ul)
+
+module HST = FStar.HyperStack.ST
+
+inline_for_extraction
+let serialize32_u16 : serializer32 #_ #_ #parse_u16 serialize_u16 =
+  fun out lo v ->
+  assert (Seq.length (serialize #_ #_ #parse_u16 serialize_u16 v) == 2);
+  let out' = B.sub out lo 2ul in
+  assert_norm (pow2 (8 `Prims.op_Multiply` 2) == 65536);
+  let h = HST.get () in
+  assert (B.live h out'); 
+  assert (B.length out' == 2);
+  assert (8 `Prims.op_Multiply` 2 <= 16);
+  assert (U16.v v < pow2 (8 `Prims.op_Multiply` 2));
+  E.n_to_be_2 U16.t 16 (E.u16 ()) v out';
+  let h' = HST.get () in
+  assert (exactly_contains_valid_data h' parse_u16 out lo v (U32.add lo 2ul))
+
+inline_for_extraction
+let serialize32_u16_fail = serializer32_fail_of_serializer #_ #_ #parse_u16 #serialize_u16 serialize32_u16 2l
+
+inline_for_extraction
+let serialize32_u32 : serializer32 #_ #_ #parse_u32 serialize_u32 =
+  fun out lo v ->
+  assert (Seq.length (serialize #_ #_ #parse_u32 serialize_u32 v) == 4);
+  let out' = B.sub out lo 4ul in
+  assert_norm (pow2 (8 `Prims.op_Multiply` 4) == 4294967296);
+  let h = HST.get () in
+  assert (B.live h out'); 
+  assert (B.length out' == 4);
+  assert (8 `Prims.op_Multiply` 4 <= 32);
+  assert (U32.v v <= pow2 32 - 1);
+  assert (U32.v v < pow2 (8 `Prims.op_Multiply` 4));
+  E.n_to_be_4 U32.t 32 (E.u32 ()) v out';
+  let h' = HST.get () in
+  assert (exactly_contains_valid_data h' parse_u32 out lo v (U32.add lo 4ul))
+
+inline_for_extraction
+let serialize32_u32_fail = serializer32_fail_of_serializer #_ #_ #parse_u32 #serialize_u32 serialize32_u32 4l
